Types/Ex1.lean
@@ -1,0 +1,105 @@
+import Types.BLang
+import Types.STLC.Typed
+import Types.STLCHOAS.Show
+
+namespace BLang.BLang1.Stx
+
+section Ex1
+def Progress : {t : _} → (a : Stx t) → ((b : _) ×' Red a b) ⊕ Val a
+  | _, .false => .inr .false
+  | _, .true => .inr .true
+  | _, .neg v =>
+    (match Progress v with
+    | .inl ⟨_, h⟩ => .inl ⟨_, .negCongr h⟩
+    | .inr .true => .inl ⟨_, .negTrue⟩
+    | .inr .false => .inl ⟨_, .negFalse⟩)
+  | _, .and a _ => (match Progress a with
+    | .inl ⟨_, h⟩=> .inl ⟨_, .andCongr h⟩
+    | .inr .true => .inl ⟨_, .andTrue⟩
+    | .inr .false => .inl ⟨_, .andFalse⟩)
+  | _, .add a b => (match Progress a, Progress b with 
+    | .inl ⟨_, h⟩, _ => .inl ⟨_, .addCongr h⟩
+    | .inr .n, .inl ⟨_, h⟩ => .inl ⟨_, .addCongr' h⟩
+    | .inr .n, .inr .n => .inl ⟨_, .add⟩)
+  | _, .lt a b =>  (match Progress a, Progress b with 
+    | .inl ⟨_, h⟩, _ => .inl ⟨_, .ltCongr h⟩
+    | .inr .n, .inl ⟨_, h⟩ => .inl ⟨_, .ltCongr' h⟩
+    | .inr (.n (n := a)), .inr (.n (n := b)) =>
+      if h : a < b then .inl ⟨_, .ltLt h⟩
+      else .inl ⟨_, .ltGe (Int.not_lt.mp h)⟩)
+  | _, .n _ => .inr .n
+
+end Ex1
+
+end BLang.BLang1.Stx
+
+namespace STLC
+
+section Ex2
+
+-- This proof is given in Types.STLC.Typed
+-- Notably this is done over de Bruijn idx'd syntax
+
+/--
+info: STLC.TySpec_replace {Γ : List Ty} {x : Ty} {body : Stx} {ty₁ : Ty} {v : Stx}
+  (hty₁ : TySpec Γ ((Stx.abs x body).app v) ty₁) : TySpec Γ (Stx.replace 0 body v) ty₁
+-/
+#guard_msgs in
+#check TySpec_replace
+
+/--
+info: STLC.Progress {Γ : List Ty} {stx : Stx} {ty : Ty} (hTy : TySpec Γ stx ty) : stx.Terminal ∨ ∃ stx', Red stx stx'
+-/
+#guard_msgs in
+#check Progress
+
+/--
+info: STLC.TypePreservation {Γ : List Ty} {e₁ e₂ : Stx} {ty : Ty} (h : Red e₁ e₂) (hTy : TySpec Γ e₁ ty) : TySpec Γ e₂ ty
+-/
+#guard_msgs in
+#check TypePreservation
+
+end Ex2
+
+section Ex4
+
+inductive DegTy : Type
+  | arr : DegTy → DegTy → DegTy
+
+def DegTy.deg : DegTy → False
+  | .arr _ v => v.deg
+
+inductive DegS : List DegTy → DegTy → Type
+  | var {Γ} (x : Fin Γ.length) : DegS Γ Γ[x]
+  | app {Γ A B} : DegS Γ (.arr A B) → DegS Γ A → DegS Γ B
+  | lam {Γ A B}  : DegS (A :: Γ) B → DegS Γ (.arr A B)
+
+def DegS.deg : {Γ : _} → {ty : _} → DegS Γ ty → False
+  | Γ, _, .var v => Γ[v].deg
+  | Γ, _, .lam x => x.deg
+  | Γ, _, .app _ x => x.deg
+
+/-
+By having no base types, the syntax of types becomes an empty type.
+This consequently means there cannot be any terms, nor instances of the type.
+Otherwise p.o. explosion.
+-/
+
+end Ex4
+
+end STLC
+
+namespace STLCHOAS
+
+section Ex5
+
+/-
+
+
+
+-/
+
+end Ex5
+
+end STLCHOAS
+
