Types/STLC/Infer.lean
@@ -1,0 +1,61 @@
+import Types.STLC.Typed
+
+namespace STLC
+
+def infer (Γ : List Ty) : Stx → Option Ty
+  | .bvar idx => Γ[idx]?
+  | .abs ty body => (infer (ty :: Γ) body).map (.arr ty ·)
+  | .app a b => do
+    let (.arr argTy retTy) ← infer Γ a | none
+    let argTy' ← infer Γ b
+    if argTy = argTy' then some retTy else none
+
+theorem infer_TySpec {Γ stx ty}
+    : infer Γ stx = .some ty ↔ TySpec Γ stx ty := match stx with
+  | .bvar idx => by simp only [infer, TySpec_bvar]
+  | .abs argTy body => by
+    constructor
+    <;> simp only [infer, Option.map_eq_some_iff, forall_exists_index, and_imp]
+    · rintro retTy h rfl
+      simp only [TySpec_abs]
+      exact infer_TySpec.mp h
+    · intro h
+      cases h
+      next retTy hBody =>
+      use retTy
+      simp only [and_true]
+      exact infer_TySpec.mpr hBody
+  | .app a b => by
+    constructor
+    <;> simp only [TySpec_app, infer, Option.bind_eq_bind, forall_exists_index, and_imp]
+    · intro x
+      obtain ⟨_|_, ap⟩ : ∃ v, infer Γ a = v := exists_eq'
+      <;> simp only [ap, Option.bind_none, Option.bind_some] at x
+      case none => contradiction
+      split at x
+      case h_2 => contradiction
+      obtain ⟨_|_, bp⟩ : ∃ v, infer Γ b = v := exists_eq'
+      <;> simp only [Option.bind_none, reduceCtorEq, Option.some.injEq, bp, Option.bind_some,
+        Option.ite_none_right_eq_some] at x
+      rcases x with ⟨rfl, rfl⟩
+      exact ⟨_, infer_TySpec.mp ap , infer_TySpec.mp bp⟩
+    · intro _ ha hb
+      rw [infer_TySpec.mpr ha, infer_TySpec.mpr hb]
+      simp only [Option.bind_some, ↓reduceIte]
+
+/-- info: 'STLC.infer_TySpec' depends on axioms: [propext, Quot.sound] -/
+#guard_msgs in
+#print axioms infer_TySpec
+
+@[simp]
+theorem infer_bvar {Γ idx} : infer Γ (.bvar idx) = Γ[idx]? := rfl
+
+@[simp]
+theorem infer_abs {Γ ty body}
+    : infer Γ (.abs ty body) = (infer (ty :: Γ) body).map (.arr ty ·) := rfl
+
+/- @[simp] -/
+/- theorem infer_app : infer Γ (.app a b) = (infer (ty :: Γ) body).map (.arr ty ·) := rfl -/
+
+end STLC
+
