Types/STLC/Red.lean
@@ -1,0 +1,17 @@
+import Types.STLC.Stx
+import Types.STLC.Red.Beta
+import Mathlib.Data.Rel
+
+namespace STLC
+
+inductive Red : Stx → Stx → Prop
+  | appl  {a a' b : Stx} : Red a a' → Red (.app a b ) (.app a' b)
+  | appr  {a b b' : Stx} : Red b b' → Red (.app a b ) (.app a b')
+  | congr {ty : Ty} {a a' : Stx} : Red a a' → Red (.abs ty a) (.abs ty a')
+  | beta  {body v : Stx} : Red (.app (.abs _ body) v) (body.β v)
+
+abbrev RedStar := Relation.ReflTransGen Red
+abbrev RedPlus := Relation.TransGen Red
+
+end STLC
+
