Types/STLC/Red/Terminal.lean
@@ -1,0 +1,89 @@
+import Types.STLC.Stx
+import Types.STLC.Red
+
+namespace STLC.Stx
+
+mutual
+inductive NonEval : Stx → Prop
+  | bvar {idx : ℕ} : NonEval (.bvar idx)
+  | app {a b : Stx} (lhs : NonEval a) (rhs : Terminal b) : NonEval (.app a b)
+
+inductive Terminal : Stx → Prop
+  | abs {ty : Ty} {a : Stx} (h : Terminal a) : Terminal (.abs ty a)
+  | nonEval {a : Stx} (h : NonEval a) : Terminal a
+end
+
+@[simp]
+theorem Terminal_abs {ty : Ty} {a : Stx} : Terminal (.abs ty a) ↔ Terminal a := by
+  constructor
+  <;> intro h
+  · cases h
+    next h => exact h
+    next h => cases h
+  · exact .abs h
+
+@[simp]
+theorem NonEval_bvar {idx : ℕ} : NonEval (.bvar idx) ↔ True := by
+  constructor <;> intro _
+  · trivial
+  · exact .bvar
+
+@[simp]
+theorem Terminal_bvar {idx : ℕ} : Terminal (.bvar idx) ↔ True := by
+  constructor <;> intro _
+  · trivial
+  · exact .nonEval .bvar
+
+@[simp]
+theorem Terminal_app {a b : Stx} : Terminal (.app a b) ↔ (NonEval a) ∧ (Terminal b) := by
+  constructor
+  <;> intro h
+  · cases h; next h =>
+    cases h; next a b =>
+    exact ⟨a, b⟩
+  · rcases h with ⟨a, b⟩
+    exact .nonEval $ .app a b
+
+@[simp]
+theorem NonEval_app {a b : Stx} : NonEval (.app a b) ↔ (NonEval a) ∧ (Terminal b) := by
+  constructor
+  <;> intro h
+  · cases h; next a b =>
+    exact ⟨a, b⟩
+  · rcases h with ⟨a, b⟩
+    exact .app a b
+
+mutual
+/-- Proof of correctness for terminal -/
+theorem Terminal_not_Red {a b : Stx} (terminal : Stx.Terminal a) : ¬Red a b := fun h =>
+  match h with
+  | .appl h => by
+    rw [Stx.Terminal_app] at terminal
+    rcases terminal with ⟨a, _⟩
+    exact NonEval_not_Red a h
+  | .appr h => by
+    rw [Stx.Terminal_app] at terminal
+    rcases terminal with ⟨_, a⟩
+    exact Terminal_not_Red a h
+  | .congr h => by
+    rw [Stx.Terminal_abs] at terminal
+    exact Terminal_not_Red terminal h
+  | .beta => by rcases terminal with (_|_|_|_)
+theorem NonEval_not_Red {a b : Stx} (terminal : Stx.NonEval a) : ¬Red a b := fun h =>
+  match h with
+  | .appl h => by
+    rw [Stx.NonEval_app] at terminal
+    rcases terminal with ⟨a, _⟩
+    exact NonEval_not_Red a h
+  | .appr h => by
+    rw [Stx.NonEval_app] at terminal
+    rcases terminal with ⟨_, a⟩
+    exact Terminal_not_Red a h
+  | .congr h => by
+    cases terminal
+  | .beta => by rcases terminal with (_|_|_)
+end
+
+end Stx
+
+end STLC
