Types/STLC/Step.lean
@@ -1,0 +1,122 @@
+import Types.STLC.Stx
+import Types.STLC.Red
+import Types.STLC.StrongNorm
+import Mathlib.Data.Rel
+import LeanScratch.Relation
+import LeanScratch.Rel2
+
+namespace STLC
+
+def step : Stx → Option Stx
+  | .bvar _ => .none
+  | .abs ty body => (step body).map (.abs ty ·)
+  | .app (.abs _ body) repl => .some $ body.β repl
+  | .app a b => match step a, step b with
+    | .none, .none => .none
+    | .some a, .none
+    | .none, .some b
+    | .some a, .some b => .some $ .app a b
+
+lemma RedPlus_congr : RedPlus body w → RedPlus (.abs ty body) (.abs ty w) :=
+  Relation.transGenMap .congr
+
+lemma RedPlus_appl : RedPlus a w → RedPlus (.app a b) (.app w b) :=
+  Relation.transGenMap (fun {x y} => @Red.appl x y b)
+
+lemma RedPlus_appr  : RedPlus a w → RedPlus (.app b a) (.app b w) :=
+  Relation.transGenMap (fun {x y} => @Red.appr x y b)
+
+theorem step_some_RedPlus (h : step main = .some a₁) : RedPlus main a₁ := 
+  match main with
+  | .bvar id => by simp only [step] at h
+  | .abs ty body => by
+    rw [step, Option.map_eq_some'] at h
+    rcases h with ⟨w, h, rfl⟩
+    exact RedPlus_congr $ step_some_RedPlus h
+  | .app a b => by
+    by_cases isAbs : ∃ ty body, a = .abs ty body
+    · rcases isAbs with ⟨ty,body, rfl⟩
+      rw [step, Option.some.injEq] at h
+      rw [←h]
+      exact .single .beta
+    · simp only [not_exists] at isAbs
+      unfold step at h
+      split at h
+      <;> try contradiction
+      next heq =>
+        simp_all only [Stx.app.injEq, false_and]
+      next heq =>
+        split at h
+        <;> simp only [Option.some.injEq] at h
+        <;> rw [←h, heq]
+        next ha _ =>
+          exact RedPlus_appl $ step_some_RedPlus ha
+        next hb =>
+          exact RedPlus_appr $ step_some_RedPlus hb
+        next ha hb =>
+          exact (RedPlus_appr $ step_some_RedPlus hb).trans (RedPlus_appl $ step_some_RedPlus ha)
+termination_by SizeOf.sizeOf main
+decreasing_by
+  all_goals simp_wf
+  <;> simp_all only [Stx.app.injEq, Option.some.injEq]
+  <;> linarith
+
+theorem step_none_terminal (h : step main = .none) : Stx.Terminal main :=
+  match main with
+  | .bvar id => .nonEval .bvar
+  | .abs ty body => by
+    simp only [step, Option.map_eq_none', Stx.Terminal_abs] at h ⊢
+    exact step_none_terminal h
+  | .app a b => by
+    by_cases isAbs : ∃ ty body, a = .abs ty body
+    · rcases isAbs with ⟨ty,body, rfl⟩
+      simp only [step] at h
+    · simp only [not_exists] at isAbs
+      unfold step at h
+      split at h
+      <;> try contradiction
+      split at h
+      <;> try contradiction
+      next heq _ _ ha hb =>
+      rw [Stx.app.injEq] at heq
+      rcases heq with ⟨haa, hbb⟩
+      simp_all only [false_implies, implies_true, Stx.Terminal_app]
+      have ha := step_none_terminal ha
+      have hb := step_none_terminal hb
+      cases ha
+      · exfalso
+        exact isAbs _ _ rfl
+      next ha => exact ⟨ha, hb⟩
+
+def full_red_direct'
+    body
+    (spec : TySpec Γ body ty)
+    (Γ' : TyArr Γ)
+    (hΓ' : TyArr.Every ArgCount.Monotonic Γ') 
+    : Stx :=
+  match h : step body with
+  | .none => body
+  | .some nBody => full_red_direct' nBody (LongTypePreservation spec ((step_some_RedPlus h).to_reflTransGen)) Γ' hΓ'
+termination_by (upperBoundRed (TySpec_CTySpec spec) Γ').naturalize
+decreasing_by
+· simp_wf
+  exact RedPlus_nat_dec hΓ' (step_some_RedPlus h) _ _
+
+def full_red_direct
+    body
+    (spec : TySpec Γ body ty)
+    : Stx :=
+  let ⟨a, b⟩ := allZeros Γ
+  full_red_direct' body spec a b
+where
+  allZeros : (Γ : List Ty) → (Γ' : TyArr Γ) ×' (TyArr.Every ArgCount.Monotonic Γ')
+    | [] => ⟨.nil, .nil⟩
+    | _ :: tl =>
+      let ⟨a, b⟩ := allZeros tl
+      ⟨.cons ArgCount.zero a, .cons ArgCount.zero_Monotonic b⟩
+
+def full_red (body : Stx) (Γ : List Ty) : Option Stx :=
+  match h : infer Γ body with
+  | some _ => full_red_direct body (infer_TySpec.mp h)
+  | none => none
+
