Types/STLC/StrongNorm.lean
@@ -1,0 +1,226 @@
+import Types.STLC.Stx
+import Types.STLC.Red
+import Types.STLC.Typed
+import Types.STLC.Infer
+import Types.STLC.StrongNorm.CTySpec
+import Types.STLC.StrongNorm.ArgCount
+import Types.STLC.StrongNorm.TyArr
+import Types.STLC.StrongNorm.upperBoundRed
+import LeanScratch.ListUtils
+
+/-
+
+# Possible ways to solve strong normalization of STLC
+
+What does it mean for something to happen 'eventually'
+
+1.  [ ] Encode terms as ordinals
+2.  [ ] Simple structural recursion
+3.  [ ] Number of unique types decrease
+4.  [ ] Encode problem as a graph, prove there are no infinite paths + cycles
+5.  [ ] Number of bound variables
+6.  [ ] Number of lambdas
+7.  [ ] Maximum bound variable decreases (eventually?)
+8.  [ ] Locations where a function can be applied decreases
+9.  [ ] Any of the above apply on a congruence level - what does this mean
+10. [ ] A solution either decreases the maximum bvar, or it removes one bvar below it
+11. [ ] 'Negative bvars' are bound variables simply used within an
+        expression, number of 'negative bvars decrease'
+12. [ ] Do any of these metrics even matter on an application level?
+13. [ ] Eventually the smallest negative bvar has to be reduced
+14. [ ] A vector of negative bvars and occurances of said negative bvars decrease
+15. [ ] The negative bvar vector looks like a CNF-ordinal
+16. [ ] The types get less arrows in them in total
+17. [ ] The level of congruance application (eventually) decreases this relates
+18. [ ] Either types will stick around, or they will (eventually) be removed
+19. [ ] Types of lambdas cannot be created, only destroyed
+20. [ ] Number of 'hot applications' decreases, number of applications
+        with a lambda at some point on the left
+21. [ ] If any of the above hold for any sub-expression (like a lhs)
+        and for a (rhs) we can dictate they might hold for the whole expr
+22. [ ] Reducability decrease, this tracks how many lambdas / bvars
+        are on the left hand side of an expression
+23. [ ] 
+24. [ ] 
+25. [ ] 
+26. [ ] 
+27. [ ] 
+
+-/
+
+namespace STLC
+
+open ArgCount in
+theorem β_lt
+    {p₁ : CTySpec Γ (.app (.abs argTy body) arg) t₁}
+    {p₂ : CTySpec Γ (body.β arg) t₁}
+    : (upperBoundRed p₂ Γ' ) < (upperBoundRed p₁ Γ') := by
+  dsimp [Stx.β] at p₂
+  cases p₁; next pRepl hBody =>
+  cases hBody; next hBody =>
+  dsimp [upperBoundRed]
+  change CTySpec ([] ++ Γ) _ _ at pRepl
+  change CTySpec ([] ++ (_ :: Γ)) _ _ at hBody
+  obtain ⟨replSz, z⟩ : ∃ replSz, upperBoundRed pRepl Γ' = replSz := exists_eq'
+  have := upperBoundRed_eq_replace (Γ₂ := []) (Γ'₂ := .nil) pRepl z hBody p₂
+  change upperBoundRed _ (TyArr.cons _ _) = _ at this
+  rw [z, this]
+  apply self_lt_addN
+  exact Nat.zero_lt_succ _
+
+open ArgCount in
+mutual
+theorem upperBoundRed_le_from_le
+  {a b : ArgCount ty} {Γ' : TyArr Γ}
+  {Γ₂' : TyArr Γ₂}
+  (h : a ≤ b)
+  (hΓ' : TyArr.Every Monotonic Γ')
+  (aMono : Monotonic a)
+  (bMono : Monotonic b)
+  (hΓ₂' : TyArr.Every Monotonic Γ₂')
+  (hTy : CTySpec (Γ₂ ++ (ty :: Γ)) body retTy)
+  : (upperBoundRed hTy (Γ₂' ++ TyArr.cons a Γ')
+    ≤ upperBoundRed hTy (Γ₂' ++ TyArr.cons b Γ'))
+    :=
+  match body with
+  | .bvar _ => by
+    cases hTy; next idx hTy =>
+    dsimp [upperBoundRed]
+    by_cases hLtIdx : idx < Γ₂.length
+    · rw [List.getElem?_append hLtIdx] at hTy
+      rw [TyArr.get_append hTy, TyArr.get_append hTy]
+      exact self_le_self
+    · rw [not_lt] at hLtIdx
+      rw [List.getElem?_append_right hLtIdx] at hTy
+      rw [TyArr.get_append_right hLtIdx hTy, TyArr.get_append_right hLtIdx hTy]
+      generalize idx - Γ₂.length = idx at hTy
+      clear *-h
+      cases idx
+      · simp only [List.getElem?_cons_zero, Option.some.injEq] at hTy
+        subst hTy
+        simp only [TyArr.get, cast_eq]
+        exact h
+      · exact self_le_self
+  | .abs _ _ => by
+    cases hTy; next ty body retTy hTy =>
+    change CTySpec ((ty :: Γ₂) ++ _ :: _) _ _ at hTy
+    change le _ _
+    simp only [le]
+    intro x xm
+    dsimp [upperBoundRed]
+    change (upperBoundRed hTy (TyArr.cons x Γ₂' ++ TyArr.cons a Γ'))
+        ≤ (upperBoundRed hTy (TyArr.cons x Γ₂' ++ TyArr.cons b Γ'))
+    exact upperBoundRed_le_from_le h hΓ' aMono bMono (.cons xm hΓ₂') hTy
+  | .app _ _ => by
+    cases hTy; next harg hfn =>
+    dsimp [upperBoundRed]
+    change le _ _
+    have hArg : (upperBoundRed harg (Γ₂' ++ TyArr.cons a Γ')) ≤ (upperBoundRed harg (Γ₂' ++ TyArr.cons b Γ')) :=
+      upperBoundRed_le_from_le h hΓ' aMono bMono hΓ₂' _
+    have hFn  : (upperBoundRed hfn (Γ₂' ++ TyArr.cons a Γ')) ≤ (upperBoundRed hfn (Γ₂' ++ TyArr.cons b Γ')) :=
+      upperBoundRed_le_from_le h hΓ' aMono bMono hΓ₂' _
+    have fnAMono : (upperBoundRed hfn (Γ₂' ++ TyArr.cons a Γ')).Monotonic :=
+      upperBoundRed_Monotonic (TyArr.Every_concat hΓ₂' (.cons aMono hΓ'))
+    have argAMono : (upperBoundRed harg (Γ₂' ++ TyArr.cons a Γ')).Monotonic :=
+      upperBoundRed_Monotonic (TyArr.Every_concat hΓ₂' (.cons aMono hΓ'))
+    have argBMono : (upperBoundRed harg (Γ₂' ++ TyArr.cons b Γ')).Monotonic :=
+      upperBoundRed_Monotonic (TyArr.Every_concat hΓ₂' (.cons bMono hΓ'))
+
+    generalize /- hFnA :  -/ upperBoundRed hfn (Γ₂' ++ TyArr.cons a Γ') = fnA at *
+    generalize /- hFnB :  -/ upperBoundRed hfn (Γ₂' ++ TyArr.cons b Γ') = fnB at *
+    generalize /- hArgA : -/ upperBoundRed harg (Γ₂' ++ TyArr.cons a Γ') = argA at *
+    generalize /- hArgB : -/ upperBoundRed harg (Γ₂' ++ TyArr.cons b Γ') = argB at *
+
+    exact le_trans
+      (addN_le_addN_right (le_congr fnAMono argAMono argBMono hFn hArg))
+      (addN_le_addN_left (Nat.succ_le_succ (le_naturalize hArg)))
+
+theorem upperBoundRed_Monotonic
+    {Γ' : TyArr Γ} {hTy : CTySpec Γ body ty}
+    (hPrevHolds : TyArr.Every Monotonic Γ')
+    : Monotonic (upperBoundRed hTy Γ') :=
+  match body, hTy with
+  | .bvar _, .bvar hTy => TyArr.Every_get hPrevHolds
+  | .abs _ _, .abs hTy => by
+    simp only [Monotonic]
+    constructor
+    · dsimp [upperBoundRed]
+      intro a b aMono bMono h
+      change upperBoundRed _ (TyArr.nil ++ (TyArr.cons _ _)) ≤ upperBoundRed _ (TyArr.nil ++ (TyArr.cons _ _))
+      change CTySpec ([] ++ _ :: _) _ _ at hTy
+      exact upperBoundRed_le_from_le h hPrevHolds aMono bMono .nil hTy
+    · intro x xm
+      exact upperBoundRed_Monotonic (.cons xm hPrevHolds)
+  | .app _ _, .app ha hb => by
+    dsimp [upperBoundRed, Monotonic, addN]
+    apply addN_Monotonic
+    have x : Monotonic (upperBoundRed ha _) := upperBoundRed_Monotonic hPrevHolds
+    simp only [Monotonic] at x
+    rcases x with ⟨_, haMR⟩
+    exact haMR (upperBoundRed hb Γ') (upperBoundRed_Monotonic hPrevHolds)
+end
+
+open ArgCount in
+theorem Red_dec
+    {Γ' : TyArr Γ}
+    (every : TyArr.Every Monotonic Γ')
+    (h : Red a b)
+    (hTyA : CTySpec Γ a ty) (hTyB : CTySpec Γ b ty)
+    : (upperBoundRed hTyB Γ') < (upperBoundRed hTyA Γ') := by
+  induction h generalizing ty Γ Γ'
+  case appl ih =>
+    cases hTyA; cases hTyB; next hap hbp _ har hbr =>
+    obtain rfl := CTySpec_unique hap har
+    obtain rfl := CTySpec_singleton hap har
+    simp only [upperBoundRed, Nat.succ_eq_add_one]
+    exact addN_lt_addN_right 
+      $ lt_sufficency (upperBoundRed_Monotonic every)
+      $ ih every hbp hbr
+  case appr ih =>
+    cases hTyA; cases hTyB; next hap hbp _ har hbr =>
+    obtain ⟨rfl, _⟩ := (Ty.arr.injEq _ _ _ _).mp $ CTySpec_unique hbp hbr
+    obtain rfl := CTySpec_singleton hbp hbr
+    simp only [upperBoundRed, Nat.succ_eq_add_one]
+    specialize (ih (Γ' := Γ') every hap har)
+    have m : Monotonic (upperBoundRed hbp Γ') := upperBoundRed_Monotonic every
+    simp only [Monotonic] at m
+    have := m.1 _ _ (upperBoundRed_Monotonic every) (upperBoundRed_Monotonic every) (le_of_lt ih)
+    exact le_trans_lt
+      (addN_le_addN_right this)
+      $ addN_lt_addN_left
+      $ Nat.add_one_lt_add_one_iff.mpr (lt_naturalize ih)
+  case congr aBody bBody ty' _ ih =>
+    cases hTyA; cases hTyB; next ha hb =>
+    intro z zMono
+    exact ih (.cons zMono every) ha hb
+  case beta =>
+    exact β_lt
+
+/-- info: 'STLC.Red_dec' depends on axioms: [propext, Classical.choice, Quot.sound] -/
+#guard_msgs in #print axioms Red_dec
+
+open ArgCount in
+theorem Red_nat_dec
+    {Γ' : TyArr Γ}
+    (every : TyArr.Every Monotonic Γ')
+    (h : Red a b)
+    (hTyA : CTySpec Γ a ty) (hTyB : CTySpec Γ b ty)
+    : (upperBoundRed hTyB Γ').naturalize < (upperBoundRed hTyA Γ').naturalize := lt_naturalize (Red_dec every h hTyA hTyB)
+
+open ArgCount in
+theorem RedPlus_nat_dec
+    {Γ' : TyArr Γ}
+    (every : TyArr.Every Monotonic Γ')
+    (h : RedPlus a b)
+    (hTyA : CTySpec Γ a ty) (hTyB : CTySpec Γ b ty)
+    : (upperBoundRed hTyB Γ').naturalize < (upperBoundRed hTyA Γ').naturalize := by
+  induction h
+  case single a => exact Red_nat_dec every a hTyA hTyB
+  case tail b c redPlus red ih =>
+    have := TySpec_CTySpec $ LongTypePreservation (CTySpec_TySpec hTyA) (Relation.TransGen.to_reflTransGen redPlus)
+    exact lt_trans (Red_nat_dec every red this hTyB) (ih this)
+
+inductive ReflTransCount (R : a → a → Prop) : a → a → ℕ → Prop
+  | refl : ReflTransCount R x x 0
+  | tail : ReflTransCount R x y n → R y z → ReflTransCount R x z n.succ
+
