Types/STLC/StrongNorm/ArgCount.lean
@@ -1,0 +1,298 @@
+import Types.STLC.Stx
+
+namespace STLC
+
+-- TODO: look into Coc to try to understand how this nonsense works
+-- It would be really neat if I could use a type function as a argument type in a mutual manor here
+
+def ArgCount : Ty → Type
+  | .arr a b  => ArgCount a → ArgCount b
+  | .direct _ => ℕ
+
+namespace ArgCount
+
+mutual
+def lt {z : Ty} (a b : ArgCount z) : Prop := match z with
+  | .direct _ => Nat.lt a b
+  | .arr _ _ => ∀ x, Monotonic x → lt (a x) (b x)
+
+-- Not really a LE as it doest satisfy le ↔ lt ∧ neq
+def le {z : Ty} (a b : ArgCount z) : Prop := match z with
+  | .direct _ => Nat.le a b
+  | .arr _ _ => ∀ x, Monotonic x → le (a x) (b x)
+
+def Monotonic {s : Ty} (v : ArgCount s) : Prop := match s with
+  | .direct _ => True
+  | .arr argTy _ =>
+    -- Might need to add the restrictions Monotonic a and Monotonic b
+    (∀ a b : ArgCount argTy, Monotonic a → Monotonic b → le a b → le (v a) (v b)) ∧
+      (∀ x : ArgCount argTy, Monotonic x → Monotonic (v x))
+end
+
+instance {z : Ty} : LT (ArgCount z) := ⟨lt⟩
+instance {z : Ty} : LE (ArgCount z) := ⟨le⟩
+
+def inc {v : Ty} (h : ArgCount v) : ArgCount v := match v with
+  | .direct _ => Nat.succ h
+  | .arr _ _ => fun a' => inc (h a')
+
+def addN {v : Ty} (h : ArgCount v) (n : ℕ) : ArgCount v := match v with
+  | .direct _ => Nat.add h n
+  | .arr _ _ => fun a' => addN (h a') n
+
+instance {v : Ty} : HAdd (ArgCount v) ℕ (ArgCount v) := ⟨addN⟩
+theorem add_def {v : Ty} {a : ArgCount v} {n : ℕ} : a + n = addN a n := rfl
+
+theorem addN_succ_inc {t : Ty} {n : ℕ} {v : ArgCount t} : addN v (n + 1) = inc (addN v n) :=
+  match t with
+  | .direct _ => rfl
+  | .arr a b => by
+    dsimp [addN, inc]
+    apply funext
+    intro v
+    rw [addN_succ_inc]
+
+theorem addN_zero {t : Ty} {v : ArgCount t} : addN v 0 = v :=
+  match t with
+  | .direct _ => rfl
+  | .arr _ _ => by
+    dsimp [addN, inc]
+    apply funext
+    intro x
+    rw [addN_zero]
+
+def zero {v : Ty} : ArgCount v := match v with
+  | .direct _ => Nat.zero
+  | .arr _ _ => fun _ => ArgCount.zero
+def naturalize {v : Ty} (h : ArgCount v) : ℕ := match v with
+  | .direct _ => h
+  | .arr _ _ => naturalize (h ArgCount.zero)
+
+@[simp]
+theorem naturalize_zero {v : Ty} : naturalize (@zero v) = 0 := match v with
+  | .direct _ => rfl
+  | .arr _ _ => by dsimp [naturalize]; exact naturalize_zero
+
+@[simp]
+theorem naturalize_inc {z : Ty}
+    (x : ArgCount z)
+    : naturalize (inc x) = (naturalize x) + 1 :=
+  match z with
+  | .direct _ => rfl
+  | .arr _ _ => by dsimp [naturalize, inc]; rw [naturalize_inc]
+
+@[simp]
+theorem naturalize_addN 
+    {ty : Ty} {n : ℕ} {a : ArgCount ty}
+    : (addN a n).naturalize = a.naturalize + n :=
+  match ty with
+  | .direct _ => rfl
+  | .arr a b => by
+    dsimp [addN, naturalize]
+    exact naturalize_addN
+
+theorem lt_trans {t : Ty} {a b c : ArgCount t} (hab : a < b) (hbc : b < c) : a < c :=
+  match t with
+  | .direct _ => by
+    change lt _ _ at hab hbc ⊢
+    simp only [lt] at hab hbc ⊢
+    exact Nat.lt_trans hab hbc
+  | .arr _ _ => by
+    change lt _ _ at hab hbc ⊢
+    simp only [lt] at hab hbc ⊢
+    intro x xm
+    exact lt_trans (hab x xm) (hbc x xm)
+
+theorem le_trans {t : Ty} {a b c : ArgCount t} (hab : a ≤ b) (hbc : b ≤ c) : a ≤ c :=
+  match t with
+  | .direct _ => by
+    change le _ _ at hab hbc ⊢
+    simp only [le] at hab hbc ⊢
+    exact Nat.le_trans hab hbc
+  | .arr _ _ => by
+    change le _ _ at hab hbc ⊢
+    simp only [le] at hab hbc ⊢
+    intro x xm
+    specialize hab x xm
+    specialize hbc x xm
+    exact le_trans hab hbc
+
+theorem le_of_lt {z : Ty} {a b : ArgCount z} : a < b → a ≤ b :=
+  match z with
+  | .direct _ => fun h => by
+    change lt _ _ at h
+    change le _ _
+    simp only [lt, Nat.lt_eq, le, Nat.le_eq] at h ⊢
+    exact Nat.le_of_succ_le h
+  | .arr _ _ => by
+    change lt _ _ → le _ _
+    simp only [lt, le]
+    exact fun h x xm => le_of_lt (h x xm)
+
+theorem self_le_self {z : Ty} {a : ArgCount z} : a ≤ a :=
+  match z with
+  | .direct _ => by
+    change le _ _
+    simp only [le, Nat.le_eq, le_refl]
+  | .arr _ _ => by
+    change le _ _
+    simp only [le]
+    intro x _
+    exact self_le_self
+
+theorem zero_Monotonic {s : Ty} : Monotonic (@zero s) := match s with
+  | .direct _ => by simp only [Monotonic]
+  | .arr _ _ => by
+    simp only [Monotonic, zero]
+    exact ⟨fun _ _ _ _ _ => self_le_self, fun _ _ => zero_Monotonic⟩
+
+theorem le_congr {f r : Ty}
+    {aF bF : ArgCount (.arr f r)}
+    {aR bR : ArgCount f}
+    (hAFMono : Monotonic aF)
+    (hARMono : Monotonic aR)
+    (hBRMono : Monotonic bR)
+    (hFLe : aF ≤ bF)
+    (hRLe : aR ≤ bR)
+    : aF aR ≤ bF bR := by
+  change le _ _ at hFLe hRLe ⊢
+  simp only [le] at hFLe hRLe
+  simp only [Monotonic] at hAFMono hARMono
+  exact le_trans (hAFMono.1 aR bR hARMono hBRMono hRLe) (hFLe bR hBRMono)
+
+theorem lt_naturalize {v : Ty} {a b : ArgCount v} (h : a < b) : naturalize a < naturalize b :=
+  match v with
+  | .direct _ => by
+    change lt _ _ at h
+    simp only [lt, naturalize] at h ⊢
+    exact h
+    /- h -/
+  | .arr _ _ => by
+    change lt _ _ at h
+    simp only [ArgCount, lt, naturalize] at a b h ⊢
+    exact lt_naturalize <| h zero zero_Monotonic
+
+theorem le_naturalize {v : Ty} {a b : ArgCount v} (h : a ≤ b) : naturalize a ≤ naturalize b :=
+  match v with
+  | .direct _ => by
+    change le _ _ at h
+    simp only [le, naturalize] at h ⊢
+    exact h
+    /- h -/
+  | .arr _ _ => by
+    change le _ _ at h
+    simp only [ArgCount, le, naturalize] at a b h ⊢
+    exact le_naturalize <| h zero zero_Monotonic
+
+@[simp]
+theorem self_lt_addN {t : Ty} {n : ℕ} {a : ArgCount t} (h : 0 < n) : a < addN a n :=
+  match t with
+  | .direct _ => by
+    change lt a (a.add n)
+    exact Nat.lt_add_of_pos_right h
+  | .arr _ _ => by
+    change lt a fun a' ↦ (a a').addN n
+    exact fun _ _ => self_lt_addN h
+
+@[simp]
+theorem addN_lt_addN_right 
+    {t : Ty} {n : ℕ} {a b : ArgCount t} (h : a < b)
+    : addN a n < addN b n := match t with
+  | .direct _ => by
+    change lt _ _ at h
+    change lt _ _
+    simp only [ArgCount, addN, lt] at a b h ⊢
+    exact Nat.add_lt_add_right h _
+  | .arr _ _ => by
+    change lt _ _ at h
+    change lt _ _
+    simp only [ArgCount, addN, lt] at a b h ⊢
+    exact fun z zMono => addN_lt_addN_right (h z zMono)
+
+@[simp]
+theorem addN_lt_addN_left
+    {t : Ty} {n : ℕ} {a b : ArgCount t} (h : a < b)
+    : addN a n < addN b n := match t with
+  | .direct _ => by
+    change Nat.lt ( _ + _) (_ + _)
+    exact Nat.add_lt_add_right h _
+  | .arr _ _ => by
+    change lt _ _
+    simp only [ArgCount, addN, lt] at a b h ⊢
+    exact fun _ hmono => addN_lt_addN_left (h _ hmono)
+
+@[simp]
+theorem addN_le_addN_right
+    {t : Ty} {n : ℕ} {a b : ArgCount t} (h : a ≤ b)
+    : (addN a n ≤ addN b n) :=
+  match t with
+  | .direct _ => by
+    change (Nat.add a n).le (Nat.add b n)
+    exact Nat.add_le_add_right h n
+  | .arr _ _ => by
+    change ∀ x, x.Monotonic → ((a x).addN n).le ((b x).addN n)
+    exact fun x xm => addN_le_addN_right (h x xm)
+
+@[simp]
+theorem addN_le_addN_left {t : Ty} {n : ℕ} {a b : ArgCount t} (h : (a ≤ b)) : addN a n ≤ addN b n :=
+  match t with
+  | .direct _ => by
+    change Nat.le (_ + _) (_ + _)
+    exact Nat.add_le_add_right h _
+  | .arr _ _ => by
+    change ∀ x, x.Monotonic → ((a x).addN n).le ((b x).addN n)
+    exact fun _ hmono => addN_le_addN_left (h _ hmono)
+
+-- I wish this could be an inductive but its too complex
+def addN_Monotonic {s : Ty} {n : ℕ} {v : ArgCount s} (h : Monotonic v)
+    : Monotonic (addN v n) := match s with
+  | .direct _ => h
+  | .arr _ _ => ⟨
+      fun a b aMono bMono hLt => addN_le_addN_right (h.1 a b aMono bMono hLt), 
+      (addN_Monotonic <| h.right · ·)
+    ⟩
+
+theorem le_addN_lt_lt
+    {t : Ty} {n m : ℕ} {a b : ArgCount t} (hLe : a ≤ b) (hLt : n < m)
+    : a.addN n < b.addN m :=
+  match t with
+  | .direct _ => by
+    change le _ _ at hLe
+    change lt _ _
+    simp only [addN, lt, le] at hLe ⊢
+    exact (Nat.add_le_add_right hLe n).trans_lt (Nat.add_lt_add_left hLt b)
+  | .arr _ _ => by
+    change le _ _ at hLe
+    change lt _ _
+    simp only [addN, lt, le] at hLe ⊢
+    exact fun x xm => le_addN_lt_lt (hLe x xm) hLt
+
+theorem lt_sufficency {f t : Ty}
+    {a b : ArgCount (.arr f t)} {c : ArgCount f}
+    (cMono : Monotonic c)
+    (h : a < b) : a c < b c := by
+  change lt _ _ at h ⊢
+  simp only [lt] at *
+  exact h c cMono
+
+theorem le_trans_lt {t : Ty}
+    {a b c : ArgCount t}
+    (h1 : a ≤ b)
+    (h2 : b < c)
+    : a < c :=
+  match t with
+  | .direct _ => by
+    change le _ _ at h1
+    change lt _ _ at h2 ⊢
+    simp only [le, lt, ArgCount] at a b c h1 h2 ⊢
+    exact Nat.lt_of_le_of_lt h1 h2
+  | .arr _ _ => by
+    change le _ _ at h1
+    change lt _ _ at h2 ⊢
+    simp only [le, lt, ArgCount] at a b c h1 h2 ⊢
+    intro x xm
+    exact le_trans_lt (h1 x xm) (h2 x xm)
+
+end ArgCount
+
+end STLC
