Types/STLC/StrongNorm/TyArr.lean
@@ -1,0 +1,108 @@
+import Types.STLC.StrongNorm.CTySpec
+import Types.STLC.StrongNorm.ArgCount
+import Mathlib.Tactic.DepRewrite
+
+namespace STLC
+
+inductive TyArr : List Ty → Type
+  | nil : TyArr []
+  | cons {hd tl} (h : ArgCount hd) (t : TyArr tl) : TyArr (hd :: tl)
+
+namespace TyArr
+
+def concat {a b} : TyArr a → TyArr b → TyArr (a ++ b)
+  | .nil, a => a
+  | .cons hd tl, v => .cons hd (concat tl v)
+
+instance {a b} : HAppend (TyArr a) (TyArr b) (TyArr (a ++ b)) := ⟨TyArr.concat⟩
+theorem cons_append {A B t} {a : TyArr A} {b : TyArr B} {z : ArgCount t}
+    : .cons z (a ++ b) = (TyArr.cons z a) ++ b := rfl
+
+@[simp]
+theorem nil_concat {Γ} {Γ' : TyArr Γ} : (TyArr.nil ++ Γ') = Γ' := rfl
+
+def get
+    {Γ}
+    (idx : Fin Γ.length)
+    (v : TyArr Γ)
+    : ArgCount Γ[idx] := match Γ, idx, v with
+  | [], idx, _ => idx.elim0
+  | _ :: _, ⟨0, _⟩, .cons hd _ => hd
+  | _ :: _, ⟨n+1, h⟩, .cons _ tl' => get ⟨n, Nat.succ_lt_succ_iff.mp h⟩ tl'
+
+theorem get_append_assoc
+    {Γ₁ Γ₂ Γ₃}
+    {Γ₁' : TyArr Γ₁} {Γ₂' : TyArr Γ₂} {Γ₃' : TyArr Γ₃}
+    {idx : Fin (Γ₁ ++ Γ₂ ++ Γ₃).length}
+    : get idx (Γ₁' ++  Γ₂' ++ Γ₃')
+    ≍ get (idx.cast (by rw [List.append_assoc])) (Γ₁' ++ (Γ₂' ++ Γ₃')) :=
+  match Γ₁, Γ₁', idx with
+  | [], .nil, x => .refl _
+  | hd :: tl, .cons hd' tl', ⟨0, _⟩ => by
+    change get _ (cons hd' (tl' ++ Γ₂' ++ Γ₃')) ≍ get _ (cons hd' (tl' ++ (Γ₂' ++ Γ₃')))
+    dsimp [get]
+    rfl
+  | hd :: tl, .cons hd' tl', ⟨n+1, h⟩ => by
+    change get _ (cons hd' (tl' ++ Γ₂' ++ Γ₃')) ≍ get _ (cons hd' (tl' ++ (Γ₂' ++ Γ₃')))
+    dsimp [get]
+    exact get_append_assoc
+
+theorem get_append
+    {Γ₁ Γ₂ idx}
+    {Γ₁' : TyArr Γ₁} {Γ₂' : TyArr Γ₂}
+    (h : idx.toNat < Γ₁.length)
+    : get idx (Γ₁' ++ Γ₂') ≍ get (idx.castLT h) Γ₁' :=
+  match Γ₁, Γ₁', idx with
+  | [], _, idx => (Nat.not_succ_le_zero idx (by grind)).elim
+  | hd :: tl, .cons hd' tl', ⟨0, _⟩ => .refl _
+  | hd :: tl, .cons hd' tl', ⟨n+1, _⟩ => by
+    dsimp [get]
+    exact get_append (Nat.succ_lt_succ_iff.mp ‹_›)
+
+theorem get_append_right
+    {Γ₁ Γ₂ idx}
+    {Γ₁' : TyArr Γ₁} {Γ₂' : TyArr Γ₂}
+    (hLe : Γ₁.length ≤ idx.toNat)
+    : get idx (Γ₁' ++ Γ₂') ≍ get ((idx.cast (by rw [List.length_append, Nat.add_comm])).subNat Γ₁.length hLe) Γ₂' :=
+  match Γ₁, Γ₁', idx with
+  | [], .nil, idx => by
+    change get _ Γ₂' ≍ _
+    rfl
+  | hd :: tl, .cons hd' tl', ⟨0, _⟩ => by simp at hLe
+  | hd :: tl, .cons hd' tl', ⟨n+1, h⟩ => by
+    change get ⟨n, _⟩ (tl' ++ Γ₂') ≍ get ⟨n + 1 - (tl.length + 1), _⟩ Γ₂'
+    dsimp only [List.length_cons, List.cons_append, Fin.toNat_eq_val, add_le_add_iff_right] at hLe
+    have : (n + 1 - (tl.length + 1)) = (n - tl.length) := Nat.add_sub_add_right n 1 tl.length
+    rw [this] at h'
+    rw [get_idx_eq_jdx h' this]
+    exact get_append_right hLe _
+
+inductive Every (p : ∀ {s}, ArgCount s → Prop) : {Γ : _} → TyArr Γ → Prop
+  | nil : Every p .nil
+  | cons {h t} (hd : p h) : Every p t → Every p (TyArr.cons h t)
+  -- | cons (hd : p h) (tl : Every p t) : Every p (TyArr.cons h t) -- for unknown reasons the line below breaks things
+  -- TODO: bug report
+
+theorem Every_get
+    {Γ idx val p}
+    {Γ' : TyArr Γ} (h : Every p Γ')
+    {hGet : Γ[idx]? = some val}
+    : p (TyArr.get hGet Γ') :=
+  match Γ, Γ', idx, h with
+  | [], .nil, _, _ => Option.noConfusion (List.getElem?_nil.symm.trans hGet)
+  | h :: t, .cons hd tl, 0, .cons hhd _ => by
+    simp only [List.getElem?_cons_zero, Option.some.injEq] at hGet
+    subst hGet
+    simp only [get, cast_eq]
+    exact hhd
+  | h :: t, .cons _ tl, n+1, .cons _ htl => Every_get htl
+
+theorem Every_concat
+    {p A B} {a : TyArr A} {b : TyArr B}
+    (h1 : Every p a) (h2 : Every p b) : Every p (a ++ b) :=
+  match h1 with
+  | .nil => h2
+  | .cons h t => .cons h (Every_concat t h2)
+
+end STLC.TyArr
+
