Types/STLC/Stx.lean
@@ -1,0 +1,28 @@
+import Mathlib.Data.Nat.PSub
+import Mathlib.Data.Rel
+import Mathlib.Data.Finset.Basic
+import Mathlib.Tactic.Linarith.Frontend
+import Mathlib.Util.WhatsNew
+
+namespace STLC
+
+inductive Ty
+  | direct (id : ℕ)   -- a unique type
+  | arr (fn arg : Ty) -- a function type
+deriving DecidableEq
+
+infixr:30 " ⇒ " => Ty.arr
+prefix:30 "↑" => Ty.direct
+
+inductive Stx
+  | bvar (id : ℕ)
+  | app  (fn arg : Stx)
+  | abs  (ty : Ty) (body : Stx)
+deriving DecidableEq
+
+/- scoped prefix:30 "λ: " => Stx.abs -/
+/- scoped prefix:30 "b:" => Stx.bvar -/
+/- scoped infixl:30 " @ " => Stx.app -/
+
+end STLC
+
