Types/STLC/Typed.lean
@@ -1,0 +1,301 @@
+import Types.STLC.Stx
+import Types.STLC.Red
+import Types.STLC.Red.Terminal
+import Mathlib.Data.Rel
+
+namespace STLC
+
+open Stx
+
+inductive TySpec : List Ty → Stx → Ty → Prop
+  | bvar {idx ty Γ} : Γ[idx]? = some ty → TySpec Γ (.bvar idx) ty
+
+  | app {Γ fn argTy retTy arg} : TySpec Γ fn (argTy ⇒ retTy) → TySpec Γ arg argTy
+      → TySpec Γ (.app fn arg) retTy
+  | abs {Γ body ty retTy} : TySpec (ty :: Γ) body retTy
+      → TySpec Γ (.abs ty body) (ty ⇒ retTy)
+
+@[simp]
+theorem TySpec_bvar {Γ idx ty} : TySpec Γ (.bvar idx) ty ↔ Γ[idx]? = some ty := by
+  constructor
+  · rintro (h|_)
+    exact h
+  · intro h
+    exact .bvar h
+
+@[simp]
+theorem TySpec_app {Γ fn arg ty} : TySpec Γ (.app fn arg) ty ↔
+  (∃ argTy, (TySpec Γ fn (argTy ⇒ ty) ∧ TySpec Γ arg argTy)) := by
+  constructor
+  · rintro (_|_)
+    next argTy a b =>
+    exact ⟨argTy, b, a⟩
+  · intro ⟨_, a, b⟩
+    exact .app a b
+
+@[simp]
+theorem TySpec_abs {Γ argTy body retTy}
+    : TySpec Γ (.abs argTy body) (argTy ⇒ retTy) ↔ (TySpec (argTy :: Γ) body retTy) := by
+  constructor
+  · rintro (_|_|a)
+    exact a
+  · exact (.abs ·)
+
+theorem TySpec_abs' {Γ argTy body z}
+    : TySpec Γ (.abs argTy body) z
+    ↔ ∃ retTy, (z = (argTy ⇒ retTy)) ∧ (TySpec (argTy :: Γ) body retTy) := by
+  constructor
+  · rintro (_|_|a)
+    rename_i retTy
+    exists retTy
+  · rintro ⟨retTy, rfl, h⟩
+    exact .abs h
+
+theorem TySpec_unique {Γ i o₁ o₂} (a : TySpec Γ i o₁) (b : TySpec Γ i o₂) : o₁ = o₂ :=
+  match i with
+  | .bvar id => by
+    cases a
+    cases b
+    next ha hb =>
+    exact (Option.some.injEq _ _).mp <| ha.symm.trans hb
+  | .app fn arg => by
+    cases a
+    cases b
+    next a argTy₁ fnTy₁ b argTy₂ fnTy₂ =>
+    exact ((Ty.arr.injEq _ _ _ _).mp <| TySpec_unique fnTy₁ fnTy₂).2
+  | .abs ty body => by
+    cases a
+    cases b
+    next a ty₁ b ty₂ =>
+    exact (Ty.arr.injEq _ _ _ _).mpr ⟨rfl, TySpec_unique ty₁ ty₂⟩
+
+theorem bvarShift_maintain_gen
+    {Γ₂ Γ body ty₂ Γ₁}
+    (h : TySpec (Γ₂ ++ Γ) body ty₂)
+    : TySpec (Γ₂ ++ Γ₁ ++ Γ) (bvarShift Γ₁.length Γ₂.length body) ty₂
+    :=
+  match body with
+  | .bvar idx => by
+    rw [List.append_assoc, bvarShift, TySpec_bvar]
+    rw [TySpec_bvar] at h
+    split
+    next lt => grind
+    next ge =>
+      rw [not_lt] at ge
+      rw [List.getElem?_append_right ge] at h
+      rw [
+        List.getElem?_append_right (ge.trans <| Nat.le_add_right _ _),
+        Nat.sub_add_comm ge,
+        List.getElem?_append_right (Nat.le_add_left Γ₁.length (idx - Γ₂.length)),
+        add_tsub_cancel_right
+      ]
+      exact h
+  | .abs ty body => by
+    rw [List.append_assoc, bvarShift, Nat.succ_eq_add_one]
+    cases h; next retTy h =>
+    rw [←List.append_assoc]
+    rw [←List.cons_append] at h
+
+    exact .abs <| bvarShift_maintain_gen h
+
+  | .app a b => by
+    rw [bvarShift]
+    cases h; next argTy ha hb =>
+
+    exact .app (bvarShift_maintain_gen hb) (bvarShift_maintain_gen ha)
+
+theorem bvarShift_maintain
+    {Γ body ty₂ Γ₁}
+    (h : TySpec Γ body ty₂)
+    : (TySpec (Γ₁ ++ Γ) (bvarShift Γ₁.length 0 body) ty₂) := by
+  change TySpec ([] ++ Γ₁ ++ Γ) (bvarShift Γ₁.length ([] : List Ty).length body) ty₂
+  exact bvarShift_maintain_gen h
+
+theorem TySpec_replace_gen
+    {Γ body arg x Γ' ty₁}
+    (argTy : TySpec Γ arg x)
+    (base : TySpec (Γ' ++ (x :: Γ)) body ty₁)
+    : TySpec (Γ' ++ Γ) (body.replace (Γ'.length) arg) ty₁ :=
+  match body with
+  | .bvar idx => by
+    rw [replace, replace.bvar, Nat.pred_eq_sub_one]
+    split
+    <;> rename_i heq
+    <;> simp only [Nat.compare_eq_eq, Nat.compare_eq_gt, Nat.compare_eq_lt] at heq
+    · cases base; next base =>
+      rw [TySpec_bvar]
+      simp only [List.getElem?_append, heq, ↓reduceIte, getElem?_pos, Option.some.injEq] at base ⊢
+      exact base
+
+    · rw [heq] at base
+      cases base; next base =>
+      rw [List.getElem?_append_right (Nat.le_refl Γ'.length), tsub_eq_zero_of_le (Nat.le_refl _),
+        List.getElem?_cons_zero, Option.some.injEq] at base
+      subst base
+      change TySpec Γ _ _ at argTy
+      exact bvarShift_maintain (Γ₁ := Γ') argTy
+
+    · cases base; next base =>
+      cases idx
+      · contradiction
+      next n =>
+      have heq : Γ'.length ≤ n := Nat.le_of_lt_succ heq
+      rw [TySpec_bvar, add_tsub_cancel_right, List.getElem?_append_right heq]
+      rw [
+        List.getElem?_append_right <| heq.trans <| Nat.le_add_right n 1,
+        Nat.sub_add_comm heq,
+        List.getElem?_cons_succ
+      ] at base
+
+      exact base
+  | .abs ty body => by
+    rw [replace, Nat.succ_eq_add_one]
+    cases base
+    next rty₁ base =>
+    rw [←List.cons_append] at base
+    exact .abs <| TySpec_replace_gen argTy base
+  | .app a b => by
+    dsimp [replace]
+    rw [TySpec_app] at base ⊢
+    rcases base with ⟨ArgTy', hFn, hArg⟩
+
+    exact ⟨_, TySpec_replace_gen argTy hFn, TySpec_replace_gen argTy hArg⟩
+
+theorem TySpec_non_Red_Terminal
+    {Γ ty a}
+    (typed : TySpec Γ a ty) (r : ∀ b, ¬Red a b)
+    : Terminal a :=
+  match a with
+  | .bvar id => .nonEval .bvar
+  | .abs ty body => by
+    by_cases h : ∃ v, Red body v
+    · rcases h with ⟨w, p⟩
+      exfalso
+      exact r (.abs ty w) (.congr p)
+    · rw [not_exists] at h
+      rcases typed with (_|_|bodyTyped)
+      exact .abs <| TySpec_non_Red_Terminal bodyTyped h
+  | .app a b => by
+    by_cases hA : ∃ v, Red a v
+    · rcases hA with ⟨w, p⟩
+      exfalso
+      exact r _ (.appl p)
+    by_cases hB : ∃ v, Red b v
+    · rcases hB with ⟨w, p⟩
+      exfalso
+      exact r _ (.appr p)
+    rw [not_exists] at hA hB
+    rcases typed with (_|⟨hFn, hArg⟩)
+    have hA := (TySpec_non_Red_Terminal hFn hA)
+    have hB := (TySpec_non_Red_Terminal hArg hB)
+    cases hA
+    · exfalso
+      exact r _ .beta
+    next h => exact .nonEval <| .app h hB
+
+theorem Terminal_iff_non_Red
+    {Γ ty a}
+    (typed : TySpec Γ a ty) : (∀ b, ¬Red a b) ↔ Terminal a
+  := ⟨TySpec_non_Red_Terminal typed, fun x _ => Terminal_not_Red x⟩
+
+theorem TySpec_replace
+    {Γ x body ty₁ v}
+    (hty₁ : TySpec Γ (.app (.abs x body) v) ty₁)
+    : TySpec Γ (body.replace 0 v) ty₁ := by
+  rw [TySpec_app] at hty₁
+  rcases hty₁ with ⟨argTy, a, argTy⟩
+  cases a
+  next a =>
+  change TySpec ([] ++ x :: Γ) _ _ at a
+  exact TySpec_replace_gen argTy a
+
+theorem TypePreservation
+    {Γ e₁ e₂ ty}
+    (h : Red e₁ e₂) (hTy : TySpec Γ e₁ ty) : TySpec Γ e₂ ty :=
+  match h, hTy with
+  | .appl h, .app ha hb => .app (TypePreservation h ha) hb
+  | .appr h, .app ha hb => .app ha (TypePreservation h hb)
+  | .congr h, .abs hTy  => .abs <| TypePreservation h hTy
+  | .beta, hTy          => TySpec_replace ‹_›
+
+theorem Progress
+    {Γ stx ty}
+    (hTy : TySpec Γ stx ty) : Terminal stx ∨ ∃ stx', Red stx stx' :=
+  match stx with
+  | .bvar id => .inl (.nonEval .bvar)
+  | .abs ty body => by
+    cases hTy; next retTy hTy =>
+    by_cases h : ∃ body', Red body body'
+    · rcases h with ⟨w, p⟩
+      right
+      use (.abs ty w)
+      exact .congr p
+    · rw [not_exists] at h
+      exact .inl <| .abs <| TySpec_non_Red_Terminal hTy h
+  | .app a b => by
+    cases hTy
+    next argTy arg fn =>
+    rw [Terminal_app]
+    cases Progress arg
+    case inr h =>
+      rcases h with ⟨w, p⟩
+      exact .inr ⟨.app a w, .appr p⟩
+    next hB =>
+    rcases Progress fn with ((_|_)|_)
+    · exact .inr ⟨_, .beta⟩
+    case inr h =>
+      rcases h with ⟨w, p⟩
+      exact .inr ⟨.app w b, .appl p⟩
+    case nonEval hA => exact .inl ⟨hA, hB⟩
+
+theorem LongTypePreservation
+    {Γ ty e e'}
+    (spec : TySpec Γ e ty) (h : RedStar e e') : TySpec Γ e' ty := by
+  induction h
+  · exact spec
+  next a ih => exact TypePreservation a ih
+
+theorem Safety
+    {Γ ty e e₁}
+    (spec : TySpec Γ e ty) (h : RedStar e e₁) : (Terminal e₁ ∨ ∃ e₂, Red e₁ e₂) := by
+  induction h
+  · exact Progress spec
+  case tail b c cont hRed ih =>
+    have tyB := LongTypePreservation spec cont
+    rcases ih with (h|h)
+    · exact ((Terminal_iff_non_Red tyB).mpr h _ hRed).elim
+    · exact Progress <| TypePreservation hRed tyB
+
+/-- info: 'STLC.Safety' depends on axioms: [propext, Classical.choice, Quot.sound] -/
+#guard_msgs in
+#print axioms Safety
+
+theorem replace_gt_Γ
+    {Γ s t idx repl}
+    (h : TySpec Γ s t) (hLe : Γ.length ≤ idx) : s.replace idx repl = s :=
+  match s with
+  | .bvar jdx => by
+    cases h; next h =>
+    have hLt : jdx < Γ.length := by grind
+    dsimp [replace, replace.bvar]
+    split
+    <;> rename_i h
+    <;> simp only [Nat.compare_eq_eq, Nat.compare_eq_lt, Nat.compare_eq_gt] at h
+    · rfl
+    · subst h
+      exact ((lt_self_iff_false _).mp (hLt.trans_le hLe)).elim
+    · exact ((lt_self_iff_false _).mp ((hLt.trans_le hLe).trans h)).elim
+  | .app a b => by
+    cases h; next argTy ha hb =>
+    simp only [replace, replace_gt_Γ ha hLe, replace_gt_Γ hb hLe]
+  | .abs ty body => by
+    cases h; next retTy h =>
+    simp only [replace, Nat.succ_eq_add_one, abs.injEq, true_and]
+    apply replace_gt_Γ h
+    simpa only [List.length_cons, add_le_add_iff_right]
+
+/-- info: 'STLC.replace_gt_Γ' depends on axioms: [propext, Classical.choice, Quot.sound] -/
+#guard_msgs in
+#print axioms replace_gt_Γ
+end STLC
+
