Types/STLCHOAS/Stx.lean
@@ -1,0 +1,31 @@
+namespace STLCHOAS
+
+universe u v
+
+inductive Ty : Type where
+  | arr   : Ty → Ty → Ty
+  | unit  : Ty
+  | empty : Ty
+  | prod  : Ty → Ty → Ty
+  | cpd   : Ty → Ty → Ty
+
+inductive Term' (rep : Ty → Type) : Ty → Type where
+  | var {t} : rep t → Term' rep t
+
+  | lam {A B} : (rep A → Term' rep B) → Term' rep (Ty.arr A B)
+  | app {A B} : Term' rep (.arr A B) → Term' rep A → Term' rep B
+
+  | unit : Term' rep .unit
+  | empty {A} : Term' rep .empty → Term' rep A
+
+  | mkP {A B} : Term' rep A → Term' rep B → Term' rep (.prod A B)
+  | fst {A B} : Term' rep (.prod A B) → Term' rep A
+  | snd {A B} : Term' rep (.prod A B) → Term' rep B
+
+  | case {A B C} : Term' rep (.cpd A B) → (rep A → Term' rep C) → (rep B → Term' rep C) → Term' rep C
+  | inl  {A B} : Term' rep A → Term' rep (.cpd A B)
+  | inr  {A B} : Term' rep B → Term' rep (.cpd A B)
+
+def Term (t : Ty) : Type 1 :=
+  {rep : Ty → Type} → Term' rep t
+
