Types/SysF/Expr/TReplCorrect.lean
@@ -1,0 +1,242 @@
+import Types.SysF.Expr.TRepl
+import Types.SysF.Expr.TRefSet
+import Types.SysF.Expr.RefSet
+import Types.SysF.Ty.ReplCorrect
+
+namespace Expr
+
+/-- Proof of correctness for tBvarShift's shifting -/
+@[simp]
+theorem tBvarUnShift_tBvarShift {shift skip s} : tBvarUnShift shift skip (tBvarShift shift skip s) = s := by
+  induction s generalizing shift skip
+  <;> simp only [tBvarShift, tBvarUnShift, Ty.bvarUnShift_bvarShift]
+  <;> grind
+
+variable {n k} in
+section
+example : tBvarShift k 0 (.id n) = (.id n)                                          := by simp [tBvarShift]
+example : tBvarShift k 0 (.lam [t|0] (.id 0)) = (.lam (.id k) $ .id 0)              := by simp [tBvarShift, Ty.bvarShift]
+example : tBvarShift k 0 (.lam [t|1] (.id 0)) = (.lam (.id (1 + k)) $ .id 0)        := by simp [tBvarShift, Ty.bvarShift]
+example : tBvarShift k 0 (.tlam (.tapp (.id 0) [t|0])) = (.tlam $ .tapp (.id 0) [t|0]) := by simp [tBvarShift, Ty.bvarShift]
+example : tBvarShift k 0 (.tlam (.tapp (.id 0) [t|1])) = (.tlam $ .tapp (.id 0) (.id $ 1 + k)) := by simp [tBvarShift, Ty.bvarShift]
+end
+
+@[simp]
+theorem tBvarShift.inv {n z} : tBvarShift 0 n z = z := by
+  induction z generalizing n
+  <;> dsimp only [tBvarShift]
+  case app fn_ih arg_ih =>
+    simp only [Expr.app.injEq]
+    exact ⟨fn_ih, arg_ih⟩
+  case lam ty body_ih =>
+    simp only [lam.injEq, Ty.bvarShift.inv, true_and]
+    exact body_ih
+  case tapp expr_ih =>
+    simp only [tapp.injEq, Ty.bvarShift.inv, and_true]
+    exact expr_ih
+  case tlam body_ih =>
+    simp only [Expr.tlam.injEq]
+    exact body_ih
+
+theorem tBvarShift_TRefSet_general {body idx skip shift} (h : TRefSet body (idx + skip)) : TRefSet (body.tBvarShift shift skip) (idx + shift + skip) :=
+  match body with
+  | .id n => by
+    simp at h
+  | .lam ty body => by
+    simp only [TRefSet_lam, tBvarShift] at h ⊢
+    cases h
+    next h => exact .inl $ Ty.bvarShift_RefSet_general h
+    next h => exact .inr $ tBvarShift_TRefSet_general h
+  | .tlam body => by
+    simp_all [tBvarShift]
+    exact tBvarShift_TRefSet_general h
+  | .app a b => by
+    simp only [TRefSet_app, tBvarShift] at h ⊢
+    cases h
+    next h => exact .inl $ tBvarShift_TRefSet_general h
+    next h => exact .inr $ tBvarShift_TRefSet_general h
+  | .tapp expr ty => by
+    simp only [TRefSet_tapp, tBvarShift] at h ⊢
+    cases h
+    next h => exact .inl $ tBvarShift_TRefSet_general h
+    next h => exact .inr $ Ty.bvarShift_RefSet_general h
+
+theorem tBvarShift_TRefSet {body idx shift} (h : TRefSet body idx) : TRefSet (body.tBvarShift shift 0) (idx + shift) :=
+  tBvarShift_TRefSet_general h
+
+theorem tBvarShift_TRefSet_general_rev {body idx shift}
+    skip (h : TRefSet (body.tBvarShift shift skip) (idx + shift + skip))
+    : TRefSet body (idx + skip) :=
+  match body with
+  | .id n => by
+    simp_all [tBvarShift]
+  | .lam ty body => by
+    simp only [tBvarShift, TRefSet_lam] at h ⊢
+    cases h
+    next h => exact .inl $ Ty.bvarShift_RefSet_general_rev skip h
+    next h => exact .inr $ tBvarShift_TRefSet_general_rev skip h
+  | .tlam body => by
+    simp only [tBvarShift, Nat.succ_eq_add_one, TRefSet_tlam] at h ⊢
+    rw [Nat.add_assoc] at h
+    exact tBvarShift_TRefSet_general_rev (skip + 1) h
+  | .app a b => by
+    simp only [tBvarShift, TRefSet_app] at h ⊢
+    cases h
+    next h => exact .inl $ tBvarShift_TRefSet_general_rev skip h
+    next h => exact .inr $ tBvarShift_TRefSet_general_rev skip h
+  | .tapp expr ty => by
+    simp only [tBvarShift, TRefSet_tapp] at h ⊢
+    cases h
+    next h => exact .inl $ tBvarShift_TRefSet_general_rev skip h
+    next h => exact .inr $ Ty.bvarShift_RefSet_general_rev skip h
+
+example {n} : TRefSet (.lam [t|0] (.id (n + 1))) 0          := .lamT .id
+example {n} : TRefSet (.tlam (.tapp (.id 0) (.id $ n+1))) n := .tlam (.tappR .id)
+
+theorem tBvarShift_TRefSet_rev
+    {body idx shift}
+    (h : TRefSet (body.tBvarShift shift 0) (idx + shift))
+    : TRefSet body idx :=
+  tBvarShift_TRefSet_general_rev 0 h
+
+theorem tBvarShift_TRefSet_general_rev' {body idx shift}
+    skip
+    (hlt : skip + shift ≤ idx)
+    (h : TRefSet (body.tBvarShift shift skip) idx)
+    : TRefSet body (idx - shift) := by
+  obtain ⟨idx', rfl⟩ := Nat.exists_eq_add_of_le hlt
+  rw [show skip + shift + idx' = idx' + shift + skip by omega] at h
+  rw [show (skip + shift + idx' - shift) = idx' + skip by omega]
+  exact tBvarShift_TRefSet_general_rev skip h
+
+theorem tBvarShift_TRefSet_general_lt_rev {body idx shift}
+    skip
+    (hlt : idx < skip + shift)
+    (h : TRefSet (body.tBvarShift shift skip) idx)
+    : TRefSet body idx :=
+  match body with
+  | .id n => by
+    simp_all [tBvarShift]
+  | .lam ty body => by
+    simp only [tBvarShift, TRefSet_lam] at h ⊢
+    cases h
+    next h => exact .inl $ Ty.bvarShift_RefSet_general_lt_rev skip hlt h
+    next h => exact .inr $ tBvarShift_TRefSet_general_lt_rev skip hlt h
+  | .tlam body => by
+    simp [tBvarShift, Nat.succ_eq_add_one, TRefSet_tlam] at h ⊢
+    exact tBvarShift_TRefSet_general_lt_rev (skip + 1) (by omega) h
+  | .app a b => by
+    simp only [tBvarShift, TRefSet_app] at h ⊢
+    cases h
+    next h => exact .inl $ tBvarShift_TRefSet_general_lt_rev skip hlt h
+    next h => exact .inr $ tBvarShift_TRefSet_general_lt_rev skip hlt h
+  | .tapp expr ty => by
+    simp only [tBvarShift, TRefSet_tapp] at h ⊢
+    cases h
+    next h => exact .inl $ tBvarShift_TRefSet_general_lt_rev skip hlt h
+    next h => exact .inr $ Ty.bvarShift_RefSet_general_lt_rev skip hlt h
+
+theorem tBvarShift_range
+    {shift skip n}
+    : {x : _}
+    → TRefSet (tBvarShift shift skip x) n
+    → (n < skip ∨ shift + skip ≤ n)
+  | .id x, h => by cases h
+  | .lam ty body, .lamT h => by
+    have := Ty.bvarShift_range h
+    grind
+  | .lam ty body, .lamB h => by
+    have := tBvarShift_range h
+    grind
+  | .tlam body, .tlam h => by
+    cases tBvarShift_range (skip := skip.succ) h
+    <;> grind
+  | .app a b, .appL h | .app a b, .appR h => by
+    have := tBvarShift_range h
+    grind
+  | .tapp expr ty, .tappL h => by
+    have := tBvarShift_range h
+    grind
+  | .tapp expr ty, .tappR h => by
+    have := Ty.bvarShift_range h
+    grind
+
+theorem tReplace_TRefSet_general_lt_rev
+    {repl : Ty}
+    {idx jdx}
+    (hlt : idx < jdx)
+    : {body : Expr} → TRefSet (body.tReplace jdx repl) idx
+    → TRefSet body idx
+  | .id x, h => by cases h
+  | .lam ty body, .lamT h => TRefSet_lam.mpr
+    <| .inl <| Ty.replace_RefSet_general_lt_rev hlt h
+  | .lam ty body, .lamB h => TRefSet_lam.mpr
+    <| .inr <| tReplace_TRefSet_general_lt_rev hlt h
+  | .tlam body, .tlam h => TRefSet_tlam.mpr
+    <| tReplace_TRefSet_general_lt_rev (Nat.add_lt_add_right hlt 1) h
+  | .app a b, .appL h => TRefSet_app.mpr
+    <| .inl <| tReplace_TRefSet_general_lt_rev hlt h
+  | .app a b, .appR h => TRefSet_app.mpr
+    <| .inr <| tReplace_TRefSet_general_lt_rev hlt h
+  | .tapp expr ty, .tappL h => TRefSet_tapp.mpr
+    <| .inl <| tReplace_TRefSet_general_lt_rev hlt h
+  | .tapp expr ty, .tappR h => TRefSet_tapp.mpr
+    <| .inr <| Ty.replace_RefSet_general_lt_rev hlt h
+
+theorem tReplace_TRefSet_general_ge_rev
+    {repl : Ty}
+    {idx jdx}
+    (hlt : jdx ≤ idx)
+    : {body : Expr} → TRefSet (body.tReplace jdx repl) idx
+    → (TRefSet body idx.succ ∨ Ty.RefSet repl (idx - jdx))
+  | .id x, h => by cases h
+  | .lam ty body, .lamT h => by
+    simp only [Nat.succ_eq_add_one, TRefSet_lam]
+    cases Ty.replace_RefSet_general_ge_rev hlt h
+    <;> simp_all
+  | .lam ty body, .lamB h => by
+    simp only [Nat.succ_eq_add_one, TRefSet_lam] at *
+    have := tReplace_TRefSet_general_ge_rev hlt h
+    grind only
+  | .tlam body, .tlam h => by
+    simp only [Nat.succ_eq_add_one, TRefSet_tlam] at *
+    have := tReplace_TRefSet_general_ge_rev (Nat.add_le_add_right hlt 1) h
+    simp_all only [Nat.reduceSubDiff]
+  | .app a b, .appL h
+  | .app a b, .appR h => by
+    simp only [Nat.succ_eq_add_one, TRefSet_app]
+    cases tReplace_TRefSet_general_ge_rev hlt h
+    <;> simp_all
+  | .tapp expr ty, .tappL h => by
+    simp only [Nat.succ_eq_add_one, TRefSet_tapp]
+    cases tReplace_TRefSet_general_ge_rev hlt h
+    <;> simp_all
+  | .tapp expr ty, .tappR h => by
+    simp only [Nat.succ_eq_add_one, TRefSet_tapp]
+    cases Ty.replace_RefSet_general_ge_rev hlt h
+    <;> simp_all
+
+theorem tBvarShift_RefSet
+    {shift skip n}
+    : {x : _}
+    → RefSet (tBvarShift shift skip x) n
+    ↔ RefSet x n
+  | .id _ => by simp [tBvarShift]
+  | .tlam _ => by
+    simp only [tBvarShift, Nat.succ_eq_add_one, RefSet_tlam]
+    exact tBvarShift_RefSet
+  | .tapp _ _ => by 
+    simp only [tBvarShift, RefSet_tapp]
+    exact tBvarShift_RefSet
+  | .lam _ _ => by
+    simp only [tBvarShift, RefSet_lam]
+    exact tBvarShift_RefSet
+  | .app _ _ => by
+    simp only [tBvarShift, RefSet_app]
+    constructor
+    <;> rintro (h|h)
+    any_goals (have := tBvarShift_RefSet.mp h; simp_all)
+    all_goals have := (tBvarShift_RefSet (shift := shift) (skip := skip)).mpr h
+    all_goals simp_all
+
+end Expr
