Types/SysF/Ty/RefSet.lean
@@ -1,0 +1,39 @@
+import Types.SysF.Ty.Stx
+
+namespace Ty
+
+-- RefSet predicate for types
+@[grind]
+inductive RefSet : Ty → Nat → Prop
+  | fnL {a b idx} : RefSet a idx → RefSet (.fn a b) idx
+  | fnR {a b idx} : RefSet b idx → RefSet (.fn a b) idx
+  | fa {body idx} : RefSet body idx.succ → RefSet (.fa body) idx
+  | id {idx} : RefSet (.id idx) idx
+
+@[simp]
+theorem RefSet_fa {body idx} : RefSet (.fa body) idx ↔ RefSet body (idx + 1) := by
+  grind
+
+@[simp]
+theorem RefSet_fn {a b idx} : RefSet (.fn a b) idx ↔ (RefSet a idx ∨ RefSet b idx) := by
+  grind
+
+@[simp]
+theorem RefSet_id {idx jdx} : RefSet (.id idx) jdx ↔ idx = jdx := by
+  grind
+
+theorem RefSet_dist {a b idx} : RefSet (.fa (.fn a b)) idx ↔ RefSet (.fa a) idx ∨ RefSet (.fa b) idx := by
+  grind
+
+instance RefSet.dec : {t : Ty} → {n : Nat} → Decidable (RefSet t n)
+  | .id x, v => if h : x = v then .isTrue <| h ▸ .id
+    else .isFalse $ by simpa
+  | .fa b, v => match @RefSet.dec b v.succ with
+    | .isTrue h => .isTrue <| .fa h
+    | .isFalse h => .isFalse <| by simpa
+  | .fn a b, v =>
+    match @RefSet.dec a v, @RefSet.dec b v with
+    | .isTrue h, _ => .isTrue <| .fnL h
+    | _, .isTrue h => .isTrue <| .fnR h
+    | .isFalse h₁, .isFalse h₂ => .isFalse $ by simp_all
+
