Types/SysFHOAS/Denote.lean
@@ -1,0 +1,23 @@
+import Types.SysFHOAS.Stx
+
+namespace SysFPHOAS
+
+universe u
+
+@[simp]
+def Type'.denote : Type' (Sort u) → Sort (u + 1)
+  | .var T => PLift T
+  | .arr t1 t2 => Type'.denote t1 → Type'.denote t2
+  | .all f => (T : Sort u) → Type'.denote (f T)
+
+@[simp]
+def Term'.denote {ty : Type' (Sort u)} : Term' (Type'.denote) ty → ty.denote
+  | .var v => v
+  | .app t1 t2 => (Term'.denote t1) (Term'.denote t2)
+  | .lam f => fun x => Term'.denote (f x)
+  | @Term'.tapp _ _ _f term1 t => (Term'.denote term1) t
+  | @Term'.tlam _ _ f g => fun x => Term'.denote (g x)
+
+def same {ty : Ty} (t1 t2 : Term ty) : Prop :=
+  Term'.denote t1 = Term'.denote t2
+
