Types/SysFHOAS/Examples.lean
@@ -1,0 +1,133 @@
+import Types.SysFHOAS.Stx
+import Types.SysFHOAS.Denote
+import Types.SysFHOAS.Show
+
+namespace SysFPHOAS
+
+universe u v
+
+-- id_type : Type
+-- id_type : ∀ α. α → α
+def id_type : Ty :=
+  Type'.all (fun α => Type'.arr (Type'.var α) (Type'.var α))
+
+-- id : id_type =  ∀ α. α → α
+-- id = Λ α. λ (x : α). x
+def system_f_id : Term id_type :=
+    Term'.tlam (fun α => Term'.lam (fun x => Term'.var x))
+
+def church_bool_type : Ty :=
+  Type'.all (fun α => Type'.arr ((Type'.var α)) (Type'.arr (Type'.var α) (Type'.var α)))
+
+def church_bool_true : Term church_bool_type :=
+  Term'.tlam (fun α  => Term'.lam (fun t => Term'.lam (fun f => Term'.var t)))
+
+def church_bool_false : Term church_bool_type :=
+  Term'.tlam (fun α => Term'.lam (fun t => Term'.lam (fun f => Term'.var f)))
+
+def church_if_type : Ty :=
+  Type'.all fun α => Type'.arr church_bool_type (Type'.arr (Type'.var α) (Type'.arr (Type'.var α) (Type'.var α)))
+
+def church_if : Term church_if_type :=
+  Term'.tlam fun α =>
+    Term'.lam fun b =>
+      Term'.lam fun t =>
+        Term'.lam fun f =>
+          Term'.app
+            (Term'.app
+              (Term'.tapp (Term'.var b) α)
+              (Term'.var t))
+            (Term'.var f)
+
+-- Λ α. λ X Y. (if α true X Y)
+def church_if_true_syntax : Term church_bool_type :=
+  fun {T} {rep} =>
+    Term'.tlam (fun α =>
+      Term'.lam (fun X =>
+        Term'.lam (fun Y =>
+          Term'.app
+            (Term'.app
+              (Term'.app
+                (Term'.tapp (church_if (T:=T) (rep:=rep)) α)
+                (church_bool_true (T:=T) (rep:=rep)))
+              (Term'.var X))
+            (Term'.var Y))))
+
+-- Λ α. λ X Y. X
+def choose_left_syntax : Term church_bool_type :=
+  Term'.tlam (fun α => Term'.lam (fun X => Term'.lam (fun Y => Term'.var X)))
+
+-- Λ α. λ X Y. (if α false X Y)
+def church_if_false_syntax : Term church_bool_type :=
+  fun {T} {rep} =>
+    Term'.tlam (fun α =>
+      Term'.lam (fun X =>
+        Term'.lam (fun Y =>
+          Term'.app
+            (Term'.app
+              (Term'.app
+                (Term'.tapp (church_if (T:=T) (rep:=rep)) α)
+                (church_bool_false (T:=T) (rep:=rep)))
+              (Term'.var X))
+            (Term'.var Y))))
+
+
+
+example : Type'.denote id_type = ((T : _) → PLift T → PLift T) := rfl
+example : Term'.denote system_f_id = (fun (x : _) (y : PLift x) => y) := rfl
+example : Type'.denote church_bool_type = ((T : _) → PLift T → PLift T → PLift T) := rfl
+example : Term'.denote church_bool_true = (fun x (t f : PLift x) => t) := rfl
+example : Term'.denote church_bool_false = (fun x (t f : PLift x) => f) := rfl
+example : Term'.denote church_if = (fun x b t f => b x t f) := rfl
+
+
+/-- info: "∀α. (α → α)" -/
+#guard_msgs in
+#eval Type'.show id_type
+
+/-- info: "(Λα. (λa.a))" -/
+#guard_msgs in
+#eval Term'.show (system_f_id)
+
+/-- info: "(Λα. (λa.(λb.a)))" -/
+#guard_msgs in
+#eval Term'.show (church_bool_true)
+
+/-- info: "(Λα. (λa.(λb.b)))" -/
+#guard_msgs in
+#eval Term'.show (church_bool_false)
+
+/-- info: "(Λα. (λa.(λb.(λc.(((a [(α → (α → α))]) b) c)))))" -/
+#guard_msgs in
+#eval Term'.show (church_if)
+
+/--
+info: "(Λα. (λa.(λb.(((((Λβ . (λc.(λd.(λe.(((c [(β  → (β  → β ))]) d) e))))) [(∀β . (β  → (β  → β )) → (α → (α → α)))]) (Λβ . (λc.(λd.c)))) a) b))))"
+-/
+#guard_msgs in
+#eval Term'.show church_if_true_syntax
+
+/--
+info: "(Λα. (λa.(λb.(((((Λβ . (λc.(λd.(λe.(((c [(β  → (β  → β ))]) d) e))))) [(∀β . (β  → (β  → β )) → (α → (α → α)))]) (Λβ . (λc.(λd.d)))) a) b))))"
+-/
+#guard_msgs in
+#eval Term'.show church_if_false_syntax
+
+@[simp]
+theorem church_if_true {A : Sort u} (X Y : PLift A) :
+    (Term'.denote church_if) A (Term'.denote church_bool_true) X Y = X := rfl
+
+@[simp]
+theorem church_if_false {A : Sort u} (X Y : PLift A) :
+    (Term'.denote church_if) A (Term'.denote church_bool_false) X Y = Y := rfl
+
+-- Λ α. λ X Y. Y
+def choose_right_syntax : Term church_bool_type :=
+  Term'.tlam (fun α => Term'.lam (fun X => Term'.lam (fun Y => Term'.var Y)))
+
+-- Denotational equivalence theorems over the syntax
+-- prove that Λ α. λ X Y. (if α true X Y) = Λ α. λ X Y. X
+theorem if_true_equiv_left : same church_if_true_syntax choose_left_syntax := rfl
+
+-- prove that Λ α. λ X Y. (if α false X Y) = Λ α. λ X Y. Y
+theorem if_false_equiv_right : same church_if_false_syntax choose_right_syntax := rfl
