Types/SysFHOAS/Show.lean
@@ -1,0 +1,25 @@
+import Types.SysFHOAS.Stx
+
+namespace SysFPHOAS
+
+def letters : List String := ["a", "b", "c", "d", "e", "f", "g"]
+def greek : List String := ["α", "β ", "γ ", "δ", "ε"]
+
+def natToLetter (i : Nat) : String := letters.getD i "z"
+def natToGreek (i : Nat) : String := greek.getD i "ζ"
+
+def Type'.show (expr : Type' String) (level : Nat := 0) : String :=
+  match expr with
+  | .var s => s
+  | .arr t1 t2 => "(" ++ Type'.show t1 level ++ " → " ++ Type'.show t2 level ++ ")"
+  | .all  f=> "∀" ++ natToGreek level ++". " ++ Type'.show (f  (natToGreek level)) (level + 1)
+
+def Term'.show {ty : Type' String} (expr : Term' (T := String) (fun _ => String) ty) (level : Nat := 0) (typelevel : Nat := 0) :   String :=
+  match expr with
+  | .var s => s
+  | .app t1 t2 => "(" ++ Term'.show t1 level typelevel ++ " " ++ Term'.show t2 level typelevel ++ ")"
+  | .lam f => "(λ" ++ natToLetter level ++ "." ++ Term'.show (f (natToLetter level)) (level + 1) typelevel ++ ")"
+  | @Term'.tapp _ _ f term1  t => "(" ++ Term'.show term1 level typelevel ++ " [" ++ Type'.show (f t) typelevel ++ "])"
+  | @Term'.tlam _ _ f g => "(Λ" ++ natToGreek typelevel ++ ". " ++ Term'.show (g (natToGreek typelevel)) level (typelevel + 1) ++ ")"
+
+
